examples/riscv/isqrt/isqrt_symb_transfScript.sml
@@ -1,0 +1,44 @@
+open HolKernel boolLib Parse bossLib;
+
+open bir_programSyntax bir_program_labelsTheory;
+open bir_immTheory bir_valuesTheory bir_expTheory;
+open bir_tsTheory bir_bool_expTheory bir_programTheory;
+
+open bir_symbLib;
+
+open isqrtTheory;
+open isqrt_specTheory;
+open isqrt_symb_execTheory;
+
+val _ = new_theory "isqrt_symb_transf";
+
+(* ------------------------------- *)
+(* BIR symbolic execution analysis *)
+(* ------------------------------- *)
+
+(* before loop *)
+
+val init_addr_1_tm = (snd o dest_eq o concl) isqrt_init_addr_1_def;
+val end_addr_1_tm = (snd o dest_eq o concl) isqrt_end_addr_1_def;
+
+val bspec_pre_1_tm = (lhs o snd o strip_forall o concl) bspec_isqrt_pre_1_def;
+val bspec_post_1_tm = (lhs o snd o strip_forall o concl) bspec_isqrt_post_1_def;
+
+val bspec_cont_1_thm =
+ bir_symb_transfer init_addr_1_tm end_addr_1_tm bspec_pre_1_tm bspec_post_1_tm
+  bir_isqrt_prog_def isqrt_birenvtyl_def
+  bspec_isqrt_pre_1_def bspec_isqrt_post_1_def isqrt_prog_vars_def
+  isqrt_symb_analysis_1_thm isqrt_bsysprecond_1_thm isqrt_prog_vars_thm;
+
+Theorem bspec_cont_isqrt_1:
+ bir_cont bir_isqrt_prog bir_exp_true
+  (BL_Address (Imm64 ^init_addr_1_tm)) {BL_Address (Imm64 ^end_addr_1_tm)} {}
+  ^bspec_pre_1_tm
+  (\l. if l = BL_Address (Imm64 ^end_addr_1_tm)
+       then ^bspec_post_1_tm
+       else bir_exp_false)
+Proof
+ rw [bir_isqrt_prog_def,bspec_cont_1_thm]
+QED
+
+val _ = export_theory ();
